Drop dependent typing for predicates
Port everything:
- Switch to saved_interp_n
- Drop indexes from `olty`, lemmas, notations etc.
- Adjust Params
- Alpha-rename `m` to `n` in cases like `{m n} -> ... dist m ...`.

theories/Dot/hkdot/sem_kind.v
@@ -1,7 +1,7 @@
 From Coq Require FunctionalExtensionality.
 From D Require Import iris_prelude proper proofmode_extra.
 From D Require Export succ_notation.
-From D Require Import saved_interp_dep asubst_intf dlang lty.
+From D Require Import saved_interp_n asubst_intf dlang lty.
 From D Require Import swap_later_impl.
 From D.Dot Require dot_lty unary_lr.
 
@@ -19,10 +19,10 @@ Module Type HoSemTypes
 
 (** A semantic kind of arity [n] induces an partial order representing
 subtyping on types of arity [n], indexed by environments. *)
-Notation sr_kind Σ n := (env → hoLtyO Σ n → hoLtyO Σ n → iPropO Σ).
-Notation sr_kindO Σ n := (env -d> hoLtyO Σ n -d> hoLtyO Σ n -d> iPropO Σ).
+Notation sr_kind Σ := (env → hoLtyO Σ → hoLtyO Σ → iPropO Σ).
+Notation sr_kindO Σ := (env -d> hoLtyO Σ -d> hoLtyO Σ -d> iPropO Σ).
 
-Definition hoLty_equiv {Σ n} (T1 T2 : hoLtyO Σ n) : iProp Σ :=
+Definition hoLty_equiv {Σ} (T1 T2 : hoLtyO Σ) : iProp Σ :=
   ∀ args v, T1 args v ↔ T2 args v.
 
 Lemma iff_sym `{PROP : bi} (A B : PROP) :
@@ -39,24 +39,24 @@ Proof.
   iApply ("H1" with "(H2 H)").
 Qed.
 
-Lemma hoLty_equiv_refl {Σ n} (T : hoLtyO Σ n) :
+Lemma hoLty_equiv_refl {Σ} (T : hoLtyO Σ) :
   ⊢ hoLty_equiv T T.
 Proof. iIntros "%args %v". by rewrite -equiv_iff. Qed.
 
-Lemma hoLty_equiv_sym {Σ n} (T1 T2 : hoLtyO Σ n) :
+Lemma hoLty_equiv_sym {Σ} (T1 T2 : hoLtyO Σ) :
   hoLty_equiv T1 T2 -∗ hoLty_equiv T2 T1.
 Proof. iIntros "H %args %v"; iApply (iff_sym with "H"). Qed.
 
-Lemma hoLty_equiv_split `{dlangG Σ} {n} args (T1 T2 : hoLtyO Σ n) :
+Lemma hoLty_equiv_split `{dlangG Σ} args (T1 T2 : hoLtyO Σ) :
   hoLty_equiv T1 T2 -∗ (T1 args ⊆ T2 args ⊆ T1 args).
 Proof. iIntros "Heq"; iSplit; iIntros "%v H"; iApply ("Heq" with "H"). Qed.
 
 
 (** * Semantic Full Kind. *)
-Record sf_kind {Σ n} := _SfKind {
-  sf_kind_sub :> sr_kind Σ n;
+Record sf_kind {Σ} := _SfKind {
+  sf_kind_sub :> sr_kind Σ;
   sf_kind_sub_ne_2 ρ : NonExpansive2 (sf_kind_sub ρ);
-  sf_kind_sub_internal_proper (T1 T2 U1 U2 : hoLtyO Σ n) ρ:
+  sf_kind_sub_internal_proper (T1 T2 U1 U2 : hoLtyO Σ) ρ:
     hoLty_equiv T1 T2 -∗
     hoLty_equiv U1 U2 -∗
     sf_kind_sub ρ T1 U1 -∗ sf_kind_sub ρ T2 U2;
@@ -74,18 +74,18 @@ Record sf_kind {Σ n} := _SfKind {
 Add Printing Constructor sf_kind.
 (* Existing Instance sf_kind_sub_ne. Using :> would create an ambiguous coercion to Funclass. *)
 #[global] Arguments sf_kind : clear implicits.
-#[global] Arguments sf_kind_sub {_ _} !_.
-#[global] Arguments _SfKind {_ _} _.
+#[global] Arguments sf_kind_sub {_} !_.
+#[global] Arguments _SfKind {_} _.
 Notation SfKind F := (_SfKind F notc_hole _ _ _ _).
 
 Declare Scope sf_kind_scope.
 Bind Scope sf_kind_scope with sf_kind.
 Delimit Scope sf_kind_scope with K.
-Notation kApp := (sf_kind_sub : sf_kind _ _ → sr_kindO _ _).
+Notation kApp := (sf_kind_sub : sf_kind _ → sr_kindO _).
 
 Section sf_kind_ofe.
-  Context {Σ} {n : nat}.
-  Notation tpred := (sf_kind Σ n).
+  Context {Σ}.
+  Notation tpred := (sf_kind Σ).
   (* Forces inserting coercions to -d>. *)
 
   Instance sf_kind_equiv : Equiv tpred := λ A B, kApp A ≡ B.
@@ -94,23 +94,23 @@ Section sf_kind_ofe.
   Proof. by apply (iso_ofe_mixin kApp). Qed.
   Canonical Structure sf_kindO := OfeT tpred sf_kind_ofe_mixin.
 
-  Lemma sf_kind_equiv_intro (K1 K2 : sf_kind Σ n) : kApp K1 ≡ kApp K2 → K1 ≡ K2.
+  Lemma sf_kind_equiv_intro (K1 K2 : sf_kind Σ) : kApp K1 ≡ kApp K2 → K1 ≡ K2.
   Proof. apply. Qed.
 End sf_kind_ofe.
 #[global] Arguments sf_kindO : clear implicits.
 
 
-Program Definition kSub {Σ n} (f : env → env) (K : sf_kind Σ n) : sf_kind Σ n :=
+Program Definition kSub {Σ} (f : env → env) (K : sf_kind Σ) : sf_kind Σ :=
   SfKind (λI ρ, K (f ρ)).
 Next Obligation.
-  move=> n f K ρ m T1 T2 HT U1 U2 HU /=; exact: sf_kind_sub_ne_2.
+  move=> Σ f K ρ n T1 T2 HT U1 U2 HU /=; exact: sf_kind_sub_ne_2.
 Qed.
 Next Obligation. intros; simpl; exact: sf_kind_sub_internal_proper. Qed.
 Next Obligation. intros; simpl; exact: sf_kind_sub_trans. Qed.
 Next Obligation. intros; simpl; exact: sf_kind_sub_quasi_refl_1. Qed.
 Next Obligation. intros; simpl; exact: sf_kind_sub_quasi_refl_2. Qed.
 
-#[global] Program Instance inhabited_sf_kind {Σ n}: Inhabited (sf_kind Σ n) :=
+#[global] Program Instance inhabited_sf_kind {Σ}: Inhabited (sf_kind Σ) :=
   populate $ SfKind (λI _ _ _, False).
 Next Obligation. done. Qed.
 Next Obligation. cbn; eauto. Qed.
@@ -118,21 +118,21 @@ Next Obligation. cbn; eauto. Qed.
 Next Obligation. cbn; eauto. Qed.
 Next Obligation. cbn; eauto. Qed.
 
-#[global] Instance ids_sf_kind {Σ n}: Ids (sf_kind Σ n) := λ _, inhabitant.
+#[global] Instance ids_sf_kind {Σ} : Ids (sf_kind Σ) := λ _, inhabitant.
 
-#[global] Instance hsubst_sf_kind {Σ n}: HSubst vl (sf_kind Σ n) :=
+#[global] Instance hsubst_sf_kind {Σ} : HSubst vl (sf_kind Σ) :=
   λ σ K, kSub (λ ρ, (σ >> ρ)) K.
 
 
-#[global] Instance sf_kind_sub_ne {Σ n m} :
-  Proper (dist m ==> (=) ==> dist m ==> dist m ==> dist m) (@sf_kind_sub Σ n).
+#[global] Instance sf_kind_sub_ne {Σ n} :
+  Proper (dist n ==> (=) ==> dist n ==> dist n ==> dist n) (@sf_kind_sub Σ).
 Proof.
   intros K1 K2 HK ρ ? <- T1 T2 HT U1 U2 HU.
   etrans; last exact: HK. by apply sf_kind_sub_ne_2.
   (* have ? := sf_kind_sub_ne_2 K1; rewrite HT HU. apply HK. *)
 Qed.
-#[global] Instance sf_kind_sub_proper {Σ n} :
-  Proper ((≡) ==> (=) ==> (≡) ==> (≡) ==> (≡)) (@sf_kind_sub Σ n).
+#[global] Instance sf_kind_sub_proper {Σ} :
+  Proper ((≡) ==> (=) ==> (≡) ==> (≡) ==> (≡)) (@sf_kind_sub Σ).
 Proof.
   intros K1 K2 HK ρ ? <- T1 T2 HT U1 U2 HU. etrans; last exact: HK.
   by apply ne_proper_2; [exact: sf_kind_sub_ne_2|..].
@@ -140,13 +140,13 @@ Proof.
   (* have Hp := !! (ne_proper_2 (K1 ρ)). *)
   (* rewrite HT HU; exact: HK. *)
 Qed.
-#[global] Instance: Params (@sf_kind_sub) 2 := {}.
+#[global] Instance: Params (@sf_kind_sub) 1 := {}.
 
-Lemma sf_kind_equivI {Σ n} (K1 K2 : sf_kindO Σ n):
+Lemma sf_kind_equivI {Σ} (K1 K2 : sf_kindO Σ):
   (∀ ρ T1 T2, K1 ρ T1 T2 ≡ K2 ρ T1 T2) ⊣⊢@{iPropI Σ} (K1 ≡ K2).
 Proof. by uPred.unseal. Qed.
 
-Lemma sf_kind_eq {Σ n} (K1 K2 : sf_kind Σ n) : sf_kind_sub K1 = sf_kind_sub K2 → K1 = K2.
+Lemma sf_kind_eq {Σ} (K1 K2 : sf_kind Σ) : sf_kind_sub K1 = sf_kind_sub K2 → K1 = K2.
 Proof.
   destruct K1, K2; cbn.
   intros ->. f_equal; exact: ProofIrrelevance.proof_irrelevance.
@@ -154,14 +154,14 @@ Qed.
 
 (* This is really properness of sf_kind_sub; but it's also proper over the
 first argument K. Maybe that's worth a wrapper with swapped arguments. *)
-Lemma sf_kind_proper {Σ n} (K : sf_kind Σ n) ρ :
+Lemma sf_kind_proper {Σ} (K : sf_kind Σ) ρ :
   Proper ((≡) ==> (≡) ==> (≡)) (K ρ).
 Proof. move=> T1 T2 HT U1 U2 HU. exact: sf_kind_sub_proper. Qed.
-Lemma sf_kind_proper' {Σ n} (K : sf_kind Σ n) ρ T1 T2 :
+Lemma sf_kind_proper' {Σ} (K : sf_kind Σ) ρ T1 T2 :
   T1 ≡ T2 → K ρ T1 T1 ≡ K ρ T2 T2.
 Proof. intros Heq. exact: sf_kind_proper. Qed.
 
-Lemma sfkind_respects `{dlangG Σ} {n} (K : sf_kind Σ n) ρ T1 T2 :
+Lemma sfkind_respects `{dlangG Σ} (K : sf_kind Σ) ρ T1 T2 :
   hoLty_equiv T1 T2 -∗ K ρ T1 T1 -∗ K ρ T2 T2.
 Proof. iIntros "#H". iApply (sf_kind_sub_internal_proper with "H H"). Qed.
 
@@ -173,51 +173,51 @@ Section sf_kind_subst.
   and only finally lift that over sf_kind. *)
   (* XXX Name. *)
 
-  #[global] Instance hsubst_sf_kind_lemmas {n} : HSubstLemmas vl (sf_kind Σ n).
+  #[global] Instance hsubst_sf_kind_lemmas : HSubstLemmas vl (sf_kind Σ).
   Proof.
     split; intros; apply sf_kind_eq; rewrite /hsubst_sf_kind/kSub/=; [|done|];
       f_ext => ρ; autosubst.
   Qed.
-  #[global] Instance rename_sf_kind n : Rename (sf_kind Σ n) := λ r K, K.|[ren r].
-  #[global] Instance sort_sf_kind n : Sort (sf_kind Σ n) := {}.
-  #[global] Instance hsubst_sf_kind_ne ρ n:
-    NonExpansive (hsubst (outer := sf_kind Σ n) ρ).
+  #[global] Instance rename_sf_kind : Rename (sf_kind Σ) := λ r K, K.|[ren r].
+  #[global] Instance sort_sf_kind : Sort (sf_kind Σ) := {}.
+  #[global] Instance hsubst_sf_kind_ne ρ :
+    NonExpansive (hsubst (outer := sf_kind Σ) ρ).
   Proof. solve_proper_ho. Qed.
 
-  #[global] Instance hsubst_sf_kind_proper ρ n:
-    Proper ((≡) ==> (≡)) (hsubst (outer := sf_kind Σ n) ρ) := ne_proper _.
+  #[global] Instance hsubst_sf_kind_proper ρ :
+    Proper ((≡) ==> (≡)) (hsubst (outer := sf_kind Σ) ρ) := ne_proper _.
 
-  Definition kSubstOne {Σ n} v (K : sf_kind Σ n) : sf_kind Σ n :=
+  Definition kSubstOne {Σ} v (K : sf_kind Σ) : sf_kind Σ :=
     kSub (λ ρ, v.[ρ] .: ρ) K.
-  Lemma kSubstOne_eq {n} (K : sf_kind Σ n) v ρ : sf_kind_sub K.|[v/] ρ = kSubstOne v K ρ.
+  Lemma kSubstOne_eq (K : sf_kind Σ) v ρ : sf_kind_sub K.|[v/] ρ = kSubstOne v K ρ.
   Proof. by rewrite /= subst_swap_base. Qed.
 
-  Definition kShift {Σ n} (K : sf_kind Σ n) : sf_kind Σ n :=
+  Definition kShift {Σ} (K : sf_kind Σ) : sf_kind Σ :=
     kSub (λ ρ, stail ρ) K.
 
   (** Analogue of [hoEnvD_subst_compose_ind]; the lemma setup here is however slightly
       simplified. *)
-  Lemma sf_kind_subst_compose {n} (K : sf_kind Σ n) ρ1 ρ2 T1 T2 :
+  Lemma sf_kind_subst_compose (K : sf_kind Σ) ρ1 ρ2 T1 T2 :
     K.|[ρ1] ρ2 T1 T2 ⊣⊢ K (ρ1 >> ρ2) T1 T2.
   Proof. done. Qed.
 
-  Lemma kShift_eq {n} (K : sf_kind Σ n) :
+  Lemma kShift_eq (K : sf_kind Σ) :
     kShift K ≡ shift K.
   Proof. intros ρ T1 T2. rewrite sf_kind_subst_compose. autosubst. Qed.
 
-  Lemma kShift_cancel {n} (K : sf_kind Σ n) v :
+  Lemma kShift_cancel (K : sf_kind Σ) v :
     (kShift K).|[v/] ≡ K.
   Proof. by rewrite kShift_eq shift_sub. Qed.
 
-  Lemma kShift_cancel' {n} (K : sf_kind Σ n) :
+  Lemma kShift_cancel' (K : sf_kind Σ) :
     K.|[up (ren (+1))].|[ids 0/] ≡ K.
   Proof. move=> ρ /=; f_equiv; autosubst. Qed.
 
-  Definition oLam {n} (τ : oltyO Σ n) : oltyO Σ n.+1 :=
+  Definition oLam (τ : oltyO Σ) : oltyO Σ :=
     Olty (λI args ρ, τ (atail args) (ahead args .: ρ)).
     (* auncurry (λ v, Olty (λ args ρ, τ args (v .: ρ))). *)
 
-  Definition _oTAppV {n} w (T : oltyO Σ n.+1) : oltyO Σ n :=
+  Definition _oTAppV w (T : oltyO Σ) : oltyO Σ :=
     Olty (λI args ρ, T (acons w.[ρ] args) ρ).
 
 End sf_kind_subst.
@@ -228,29 +228,29 @@ Notation oTAppV T w := (_oTAppV w T).
 Section utils.
   Context `{dlangG Σ}.
 
-  #[global] Instance _oTAppV_ne n v: NonExpansive (_oTAppV (Σ := Σ) (n := n) v).
+  #[global] Instance _oTAppV_ne v: NonExpansive (_oTAppV (Σ := Σ) v).
   Proof. solve_proper_ho. Qed.
-  #[global] Instance _oTAppV_proper n v:
-    Proper ((≡) ==> (≡)) (_oTAppV (Σ := Σ) (n := n) v) := ne_proper _.
+  #[global] Instance _oTAppV_proper v:
+    Proper ((≡) ==> (≡)) (_oTAppV (Σ := Σ) v) := ne_proper _.
 
-  #[global] Instance oLam_ne n : NonExpansive (oLam (Σ := Σ) (n := n)).
+  #[global] Instance oLam_ne : NonExpansive (oLam (Σ := Σ)).
   Proof. solve_proper_ho. Qed.
 
-  #[global] Instance oLam_proper n :
-    Proper ((≡) ==> (≡)) (oLam (Σ := Σ) (n := n)) := ne_proper _.
+  #[global] Instance oLam_proper :
+    Proper ((≡) ==> (≡)) (oLam (Σ := Σ)) := ne_proper _.
 
-  Lemma oTAppV_subst {n} (T : olty Σ n.+1) v ρ :
+  Lemma oTAppV_subst (T : olty Σ) v ρ :
     (oTAppV T v).|[ρ] ≡ oTAppV T.|[ρ] v.[ρ].
   Proof.
     move=> ???/=.
     by rewrite /hsubst /hsubst_hoEnvD subst_comp.
   Qed.
 
-  Lemma envApply_oTAppV_eq n (T : olty Σ n.+1) v ρ :
+  Lemma envApply_oTAppV_eq (T : olty Σ) v ρ :
     envApply (oTAppV T v) ρ ≡ acurry (envApply T ρ) v.[ρ].
   Proof. done. Qed.
 
-  Definition sr_kintv (L U : oltyO Σ 0) : sr_kind Σ 0 := λI ρ φ1 φ2,
+  Definition sr_kintv (L U : oltyO Σ) : sr_kind Σ := λI ρ φ1 φ2,
     oClose L ρ ⊆ oClose φ1 ⊆ oClose φ2 ⊆ oClose U ρ.
 
   Lemma sr_kintv_refl L U ρ φ :
@@ -259,7 +259,7 @@ Section utils.
     by rewrite /sr_kintv (bi_emp_valid_True subtype_refl) (left_id True)%I.
   Qed.
 
-  Lemma sr_kintv_respects_hoLty_equiv_1 {T1 T2} (L U : olty Σ 0) U1 ρ :
+  Lemma sr_kintv_respects_hoLty_equiv_1 {T1 T2} (L U : olty Σ) U1 ρ :
     hoLty_equiv T1 T2 -∗ sr_kintv L U ρ T1 U1 -∗ sr_kintv L U ρ T2 U1.
   Proof.
     rewrite !(hoLty_equiv_split anil).
@@ -268,7 +268,7 @@ Section utils.
     by iApply (subtype_trans with "HT2 HM").
   Qed.
 
-  Lemma sr_kintv_respects_hoLty_equiv_2 {U1 U2} (L U : olty Σ 0) T1 ρ :
+  Lemma sr_kintv_respects_hoLty_equiv_2 {U1 U2} (L U : olty Σ) T1 ρ :
     hoLty_equiv U1 U2 -∗ sr_kintv L U ρ T1 U1 -∗ sr_kintv L U ρ T1 U2.
   Proof.
     rewrite !(hoLty_equiv_split anil).
@@ -278,7 +278,7 @@ Section utils.
   Qed.
 End utils.
 
-Program Definition sf_kintv `{dlangG Σ} (L U : oltyO Σ 0) : sf_kind Σ 0 :=
+Program Definition sf_kintv `{dlangG Σ} (L U : oltyO Σ) : sf_kind Σ :=
   SfKind (sr_kintv L U).
 Next Obligation. cbn; solve_proper_ho. Qed.
 Next Obligation.
@@ -300,17 +300,17 @@ Qed.
 
 Notation sf_star := (sf_kintv oBot oTop).
 
-Lemma acurry_respects_hoLty_equiv {Σ n} {T1 T2 : hoLty Σ n.+1} arg :
+Lemma acurry_respects_hoLty_equiv {Σ} {T1 T2 : hoLty Σ} arg :
   hoLty_equiv T1 T2 -∗ hoLty_equiv (acurry T1 arg) (acurry T2 arg).
 Proof. by iIntros "H %%". Qed.
 
-Program Definition sf_kpi `{dlangG Σ} {n} (S : oltyO Σ 0) (K : sf_kind Σ n) :
-  sf_kind Σ n.+1 := SfKind
+Program Definition sf_kpi `{dlangG Σ} (S : oltyO Σ) (K : sf_kind Σ) :
+  sf_kind Σ := SfKind
     (λI ρ φ1 φ2,
       ∀ arg, S anil ρ arg →
       K (arg .: ρ) (acurry φ1 arg) (acurry φ2 arg)).
 Next Obligation.
-  move=> Σ ? ? n S K ρ m T1 T2 HT U1 U2 HU /=.
+  move=> Σ ? ? S K ρ n T1 T2 HT U1 U2 HU /=.
   f_equiv => ?; f_equiv.
   by apply sf_kind_sub_ne_2; apply acurry_ne.
 Qed.
@@ -339,12 +339,12 @@ Section kinds_types.
   #[global] Instance sf_kintv_proper :
     Proper ((≡) ==> (≡) ==> (≡)) (sf_kintv (Σ := Σ)) := ne_proper_2 _.
 
-  #[global] Instance sf_kpi_ne n : NonExpansive2 (sf_kpi (Σ := Σ) (n := n)).
+  #[global] Instance sf_kpi_ne : NonExpansive2 (sf_kpi (Σ := Σ)).
   Proof. solve_proper_ho. Qed.
-  #[global] Instance sf_kpi_proper {n} :
-    Proper ((≡) ==> (≡) ==> (≡)) (sf_kpi (Σ := Σ) (n := n)) := ne_proper_2 _.
+  #[global] Instance sf_kpi_proper :
+    Proper ((≡) ==> (≡) ==> (≡)) (sf_kpi (Σ := Σ)) := ne_proper_2 _.
 
-  Lemma kShift_sf_kpi_eq {n} S (K : sf_kind Σ n) :
+  Lemma kShift_sf_kpi_eq S (K : sf_kind Σ) :
     kShift (sf_kpi S K) ≡ sf_kpi (oShift S) K.|[up (ren (+1))].
   Proof.
     move=> ???/=; properness; first done; f_equiv.
@@ -352,11 +352,11 @@ Section kinds_types.
   Qed.
 
   (** Subtle: this requires [ahead] to be total! *)
-  Lemma sTEq_oLam_oLaterN {n} (τ : oltyO Σ n) m :
+  Lemma sTEq_oLam_oLaterN (τ : oltyO Σ) m :
     oLaterN m (oLam τ) ≡ oLam (oLaterN m τ).
   Proof. done. Qed.
 
-  Lemma sTEq_oTAppV_oLaterN {n} (τ : oltyO Σ n.+1) m v:
+  Lemma sTEq_oTAppV_oLaterN (τ : oltyO Σ) m v:
     oLaterN m (oTAppV τ v) ≡ oTAppV (oLaterN m τ) v.
   Proof. done. Qed.
 End kinds_types.
@@ -366,11 +366,11 @@ Module SKindSyn.
 (* XXX rename *)
 (** An inductive representation of gHkDOT semantic kinds. *)
 Inductive s_kind {Σ} : nat → Type :=
-  | s_kintv : oltyO Σ 0 → oltyO Σ 0 → s_kind 0
-  | s_kpi n : oltyO Σ 0 → s_kind n → s_kind n.+1.
+  | s_kintv : oltyO Σ → oltyO Σ → s_kind 0
+  | s_kpi n : oltyO Σ → s_kind n → s_kind n.+1.
 #[global] Arguments s_kind: clear implicits.
 
-Inductive s_kind_rel {Σ} {R : relation (oltyO Σ 0)} : ∀ {n : nat}, relation (s_kind Σ n) :=
+Inductive s_kind_rel {Σ} {R : relation (oltyO Σ)} : ∀ {n : nat}, relation (s_kind Σ n) :=
   | s_kintv_rel L1 L2 U1 U2 :
     R L1 L2 → R U1 U2 →
     s_kind_rel (s_kintv L1 U1) (s_kintv L2 U2)
@@ -381,7 +381,7 @@ Inductive s_kind_rel {Σ} {R : relation (oltyO Σ 0)} : ∀ {n : nat}, relation 
 #[global] Arguments s_kind_rel {_} R _ _ _.
 
 Section s_kind_rel_prop.
-  Context `{R : relation (oltyO Σ 0)}.
+  Context `{R : relation (oltyO Σ)}.
   #[global] Instance s_kind_rel_refl n `(!Reflexive R) : Reflexive (s_kind_rel R n).
   Proof. elim; constructor; eauto. Qed.
 
@@ -418,7 +418,7 @@ End s_kind_ofe.
 Canonical Structure s_kindO Σ n := OfeT (s_kind Σ n) s_kind_ofe_mixin.
 
 Section s_kind_rel_proper.
-  Context `{R : relation (oltyO Σ 0)}.
+  Context `{R : relation (oltyO Σ)}.
 
   #[global] Instance s_kintv_proper_s_kind_rel : Proper (R ==> R ==> s_kind_rel R 0) s_kintv.
   Proof. constructor; auto. Qed.
@@ -464,7 +464,7 @@ Proof.
       by rewrite !hsubst_comp ?IHK ?up_comp.
 Qed.
 
-Fixpoint s_kind_to_sf_kind `{dlangG Σ} {n} (K : s_kind Σ n) : sf_kind Σ n :=
+Fixpoint s_kind_to_sf_kind `{dlangG Σ} {n} (K : s_kind Σ n) : sf_kind Σ :=
   match K with
   | s_kintv L U => sf_kintv L U
   | s_kpi S K => sf_kpi S (s_kind_to_sf_kind K)
@@ -483,7 +483,7 @@ Section s_kind_to_sf_kind.
   #[global] Instance s_kind_to_sf_kind_proper {n} :
     Proper ((≡) ==> (≡)) (s_kind_to_sf_kind (n := n)) := ne_proper _.
 
-  Lemma s_kind_equiv_intro {n} (K1 K2 : s_kind Σ n) : K1 ≡ K2 → s_to_sf K1 ≡@{sf_kind _ _} s_to_sf K2.
+  Lemma s_kind_equiv_intro {n} (K1 K2 : s_kind Σ n) : K1 ≡ K2 → s_to_sf K1 ≡@{sf_kind _} s_to_sf K2.
   Proof. apply s_kind_to_sf_kind_proper. Qed.
 
   Lemma s_kind_to_sf_kind_subst {n} (K : s_kind Σ n) ρ :
@@ -495,7 +495,7 @@ Section s_kind_to_sf_kind.
   Qed.
 End s_kind_to_sf_kind.
 
-Fixpoint ho_intv {Σ n} (K : s_kindO Σ n) : oltyO Σ n → oltyO Σ n → s_kindO Σ n :=
+Fixpoint ho_intv {Σ n} (K : s_kindO Σ n) : oltyO Σ → oltyO Σ → s_kindO Σ n :=
   match K with
   | s_kintv _ _ =>
     λ T1 T2, s_kintv T1 T2
@@ -554,15 +554,15 @@ Implicit Types
          (v w : vl) (e : tm) (d : dm) (ds : dms) (p : path)
          (ρ : var → vl) (l : label).
 
-Definition sem_kind_path_repl {Σ n} p q (K1 K2 : sf_kind Σ n) : Prop :=
+Definition sem_kind_path_repl {Σ} p q (K1 K2 : sf_kind Σ) : Prop :=
   ∀ ρ T1 T2, alias_paths p.|[ρ] q.|[ρ] → K1 ρ T1 T2 ≡ K2 ρ T1 T2.
 Notation "K1 ~sKd[ p := q  ]* K2" :=
   (sem_kind_path_repl p q K1 K2) (at level 70).
 
-Definition oDTMemK `{!dlangG Σ} {n} (K : sf_kind Σ n) : dltyO Σ :=
-  oDTMemRaw n (λI ρ ψ, K ρ (packHoLtyO ψ) (packHoLtyO ψ)).
+Definition oDTMemK `{!dlangG Σ} (K : sf_kind Σ) : dltyO Σ :=
+  oDTMemRaw (λI ρ ψ, K ρ (packHoLtyO ψ) (packHoLtyO ψ)).
 
-Definition oDTMemSpec `{!dlangG Σ} (L U : oltyO Σ 0) : dltyO Σ :=
+Definition oDTMemSpec `{!dlangG Σ} (L U : oltyO Σ) : dltyO Σ :=
   oDTMemK (sf_kintv L U).
 
 Lemma oDTMemSpec_oDTMem_eq `{!dlangG Σ} L U : oDTMemSpec L U ≡ oDTMem L U.
@@ -570,19 +570,19 @@ Proof.
   move=> ρ d /=; f_equiv=> ψ; f_equiv. apply sr_kintv_refl.
 Qed.
 
-Definition cTMemK `{!dlangG Σ} {n} l (K : sf_kind Σ n) : clty Σ := dty2clty l (oDTMemK K).
+Definition cTMemK `{!dlangG Σ} l (K : sf_kind Σ) : clty Σ := dty2clty l (oDTMemK K).
 Notation oTMemK l K := (clty_olty (cTMemK l K)).
 
 Definition oDTMemAnyKind `{!dlangG Σ} : dltyO Σ := Dlty (λI ρ d,
-  ∃ n (ψ : hoD Σ n), d ↗n[ n ] ψ).
+  ∃ (ψ : hoD Σ), d ↗n ψ).
 Definition cTMemAnyKind `{!dlangG Σ} l : clty Σ := dty2clty l oDTMemAnyKind.
 Notation oTMemAnyKind l := (clty_olty (cTMemAnyKind l)).
 
-Program Definition kpSubstOne `{!dlangG Σ} {n} p (K : sf_kind Σ n) : sf_kind Σ n :=
+Program Definition kpSubstOne `{!dlangG Σ} p (K : sf_kind Σ) : sf_kind Σ :=
   SfKind
     (λI ρ T1 T2, path_wp p.|[ρ] (λ v, K (v .: ρ) T1 T2)).
 Next Obligation.
-  move=> Σ ? n K v ρ m T1 T2 HT U1 U2 HU /=. f_equiv=>?. exact: sf_kind_sub_ne_2.
+  move=> Σ ? p K v m T1 T2 HT U1 U2 HU /=. f_equiv=>?. exact: sf_kind_sub_ne_2.
 Qed.
 Next Obligation.
   iIntros "* #Heq1 #Heq2 H". iApply (path_wp_wand with "H");
@@ -603,59 +603,59 @@ Next Obligation.
 Qed.
 Notation "K .sKp[ p /]" := (kpSubstOne p K) (at level 65).
 
-Definition oTApp `{!dlangG Σ} {n} (T : oltyO Σ n.+1) (p : path) : oltyO Σ n :=
+Definition oTApp `{!dlangG Σ} (T : oltyO Σ) (p : path) : oltyO Σ :=
   Olty (λ args ρ v, path_wp p.|[ρ] (λ w, T (acons w args) ρ v)).
 
 Section proper_eq.
   Context `{!dlangG Σ}.
 
-  #[global] Instance oDTMemK_ne n : NonExpansive (oDTMemK (Σ := Σ) (n := n)).
+  #[global] Instance oDTMemK_ne : NonExpansive (oDTMemK (Σ := Σ)).
   Proof. solve_proper_ho. Qed.
-  #[global] Instance oDTMemK_proper n :
-    Proper ((≡) ==> (≡)) (oDTMemK (Σ := Σ) (n := n)) := ne_proper _.
-  #[global] Instance cTMemK_ne n l : NonExpansive (cTMemK (Σ := Σ) (n := n) l).
+  #[global] Instance oDTMemK_proper :
+    Proper ((≡) ==> (≡)) (oDTMemK (Σ := Σ)) := ne_proper _.
+  #[global] Instance cTMemK_ne l : NonExpansive (cTMemK (Σ := Σ) l).
   Proof. solve_proper_ho. Qed.
-  #[global] Instance cTMemK_proper n l :
-    Proper ((≡) ==> (≡)) (cTMemK (Σ := Σ) (n := n) l) := ne_proper _.
+  #[global] Instance cTMemK_proper l :
+    Proper ((≡) ==> (≡)) (cTMemK (Σ := Σ) l) := ne_proper _.
 
-  Lemma cTMemK_eq {n} l (K : sf_kind Σ n) d ρ :
+  Lemma cTMemK_eq l (K : sf_kind Σ) d ρ :
     cTMemK l K ρ [(l, d)] ⊣⊢ oDTMemK K ρ d.
   Proof. apply dty2clty_singleton. Qed.
 
-  Lemma oTMemK_eq n l K args ρ v :
+  Lemma oTMemK_eq l K args ρ v :
     oTMemK l K args ρ v ⊣⊢
-    ∃ ψ d, ⌜v @ l ↘ d⌝ ∧ d ↗n[ n ] ψ ∧ K ρ (packHoLtyO ψ) (packHoLtyO ψ).
+    ∃ ψ d, ⌜v @ l ↘ d⌝ ∧ d ↗n ψ ∧ K ρ (packHoLtyO ψ) (packHoLtyO ψ).
   Proof. apply bi_exist_nested_swap. Qed.
 
   Lemma cTMemAnyKind_eq l d ρ :
     cTMemAnyKind l ρ [(l, d)] ⊣⊢ oDTMemAnyKind ρ d.
   Proof. apply dty2clty_singleton. Qed.
 
-  Lemma cTMemK_subst {n} l (K : sf_kind Σ n) ρ :
+  Lemma cTMemK_subst l (K : sf_kind Σ) ρ :
     (oTMemK l K).|[ρ] = oTMemK l K.|[ρ].
   Proof. done. Qed.
 
-  Lemma kpSubstOne_eq {n} (K : sf_kind Σ n) v :
+  Lemma kpSubstOne_eq (K : sf_kind Σ) v :
     K.|[v/] ≡ K .sKp[ pv v /].
   Proof. move=> ???. by rewrite /= path_wp_pv_eq subst_swap_base. Qed.
 
-  Lemma oTApp_pv {n} (T : oltyO Σ n.+1) w :
+  Lemma oTApp_pv (T : oltyO Σ) w :
     oTApp T (pv w) ≡ oTAppV T w.
   Proof. intros ???. by rewrite /= path_wp_pv_eq. Qed.
 
-  Lemma sTEq_oTApp_pv_oLaterN {n} (τ : oltyO Σ n.+1) m v:
+  Lemma sTEq_oTApp_pv_oLaterN (τ : oltyO Σ) m v:
     oLaterN m (oTApp τ (pv v)) ≡ oTApp (oLaterN m τ) (pv v).
   Proof. by rewrite !oTApp_pv. Qed.
 
-  Lemma sTEq_oTApp_oLaterN {n} (τ : oltyO Σ n.+1) m p args ρ v:
+  Lemma sTEq_oTApp_oLaterN (τ : oltyO Σ) m p args ρ v:
     oTApp (oLaterN m τ) p args ρ v ⊢ oLaterN m (oTApp τ p) args ρ v.
   Proof. by rewrite /= path_wp_laterN_swap. Qed.
 
-  Lemma sTEq_Beta {n} (T : oltyO Σ n) p :
+  Lemma sTEq_Beta (T : oltyO Σ) p :
     oTApp (oLam T) p ≡ T .sTp[ p /].
   Proof. done. Qed.
 
-  Lemma sTEq_BetaV {n} (T : oltyO Σ n) v :
+  Lemma sTEq_BetaV (T : oltyO Σ) v :
     oTAppV (oLam T) v ≡ T.|[v/].
   Proof. move => args ρ w /=. by rewrite subst_swap_base. Qed.
 
