theories/DSub/lr/ds_unary_lr.v
@@ -1,4 +1,4 @@
-From D Require Export iris_prelude saved_interp_dep.
+From D Require Export iris_prelude saved_interp_n.
 From D Require Import persistence.
 From D.DSub Require Import ds_syn.
 From D.DSub Require Import ds_ty_interp_subst_lemmas.
